fixed preamble to awkward example, defined the invariant needed for the malloc'ed region, fixed specs to awkward example

theories/examples/awkward_example.v
@@ -10,10 +10,11 @@ Section awkward_example.
             MonRef: MonRefG (leibnizO _) CapR_rtc Σ,
             Heap: heapG Σ}.
 
-   (* choose a special register for the environment *)
+   (* choose a special register for the environment and adv pointer *)
    (* note that we are here simplifying the environment to simply point to one location *)      
    Definition r_env : RegName := r_t30.
-   
+   Definition r_adv : RegName := r_t31.
+   Definition r_self : RegName := r_t29.
    
    Ltac isWithinBounds := rewrite /withinBounds; apply andb_true_iff; split; apply Z.leb_le; simpl; auto.
    
@@ -44,42 +45,154 @@ Section awkward_example.
     
    (* Recall that the malloc subroutine lies in b_m e_m *)
 
-   Definition awkward_preamble_instrs offset_to_awkward :=
-     malloc_subroutine r_env 1 ++
-     [move_r r_t3 PC;
-     lea_z r_t3 offset_to_awkward;
-     jmp r_t3].
+   (* assume that r1 contains an executable pointer to the malloc subroutine *)
+   Definition awkward_preamble_instrs r1 offset_to_awkward :=
+     [move_r r_t0 PC;
+     lea_z r_self 1;
+     jmp r1;
+     move_r r_self PC;
+     lea_z r_self offset_to_awkward;
+     jmp r_self].
    
    (* assume r1 contains an executable pointer to adversarial code *)
-   Definition awkward_instrs (r1 : RegName) epilogue_off flag_off :=
+   (* assume r0 contains an executable pointer to the awkward example *)
+   Definition awkward_instrs (r0 r1 : RegName) epilogue_off flag_off :=
      [store_z r_env 0] ++
+     push_r_instrs r_stk r_env ++
+     push_r_instrs r_stk r0 ++
+     push_r_instrs r_stk r1 ++
      scall_prologue_instrs epilogue_off r1 ++
      [jmp r1;
      sub_z_z r_t1 0 7;
-     lea_r r_stk r_t1;
-     store_z r_env 1] ++
+     lea_r r_stk r_t1] ++
+     pop_instrs r_stk r1 ++
+     pop_instrs r_stk r0 ++
+     pop_instrs r_stk r_env ++
+     [store_z r_env 1] ++
+     push_r_instrs r_stk r_env ++
+     push_r_instrs r_stk r0 ++
      scall_prologue_instrs epilogue_off r1 ++
      [jmp r1;
      sub_z_z r_t1 0 7;
-     lea_r r_stk r_t1;
+     lea_r r_stk r_t1] ++
+     pop_instrs r_stk r0 ++
+     pop_instrs r_stk r_env ++
      (* assert that the cap in r_env points to 1 *)
-     load_r r1 r_env;
+     [load_r r1 r_env;
      move_r r_t1 PC;
      lea_z r_t1 5; (* offset to assertion failure *)
      sub_r_z r1 r1 1;
      jnz r_t1 r1;
-     halt;
+     jmp r0;
      (* failure *)
      move_r r_t1 PC;
      lea_z r_t1 flag_off;
      store_z r_t1 1;
-     halt]. 
-  
-   Definition awkward_preamble a p offset_to_awkward :=
-     ([∗ list] a_i;w_i ∈ a;(awkward_preamble_instrs offset_to_awkward), a_i ↦ₐ[p] w_i)%I.
+     halt].
+
    
-   Definition awkward_example (a : list Addr) (p : Perm) (r1 : RegName) epilogue_off flag_off : iProp Σ :=
-     ([∗ list] a_i;w_i ∈ a;(awkward_instrs r1 epilogue_off flag_off), a_i ↦ₐ[p] w_i)%I.
+  
+   Definition awkward_preamble a p r1 offset_to_awkward :=
+     ([∗ list] a_i;w_i ∈ a;(awkward_preamble_instrs r1 offset_to_awkward), a_i ↦ₐ[p] w_i)%I.
+   
+   Definition awkward_example (a : list Addr) (p : Perm) (r0 r1 : RegName) epilogue_off flag_off : iProp Σ :=
+     ([∗ list] a_i;w_i ∈ a;(awkward_instrs r0 r1 epilogue_off flag_off), a_i ↦ₐ[p] w_i)%I.
+
+   
+   Definition awk_inv i a :=
+     (∃ x:bool, sts_state_loc i x
+           ∗ if x
+             then a ↦ₐ[RW] inl 1%Z
+             else a ↦ₐ[RW] inl 0%Z)%I.
+
+   Definition awk_rel_pub := λ a b, a = false ∨ b = true.
+   Definition awk_rel_priv := λ (a b : bool), True.
+
+   (* the following spec is for the preamble to the awkward example. It allocates the invariant on the malloc'ed region *)
+   Lemma g1_spec φ W pc_p pc_g pc_b pc_e (* PC *)
+         g1_addrs offset_to_awkward (* g1 *)
+         a_first a_last a_cont (* special adresses *) :
+
+     (* PC assumptions *)
+     isCorrectPC (inr ((pc_p,pc_g),pc_b,pc_e,a_first)) ∧
+     isCorrectPC (inr ((pc_p,pc_g),pc_b,pc_e,a_last)) →
+     
+     (* Program adresses assumptions *)
+     contiguous g1_addrs ->
+     g1_addrs !! 0 = Some a_first ∧ list.last g1_addrs = Some a_last ->
+
+     (* Address assumptions *)
+     (a_first + (3 + offset_to_awkward))%a = Some a_cont ->
+
+     (PC ↦ᵣ inr ((pc_p,pc_g),pc_b,pc_e,a_first)
+      ∗ r_t1 ↦ᵣ inr (E,Global,b_m,e_m,a_m)
+      ∗ (∃ wsr, [∗ list] r_i;w_i ∈ list_difference all_registers [PC;r_t1]; wsr, r_i ↦ᵣ w_i)
+      ∗ awkward_preamble g1_addrs pc_p r_t1 offset_to_awkward
+      ∗ region W
+      ∗ sts_full_world sts_std W
+      ∗ ▷ (PC ↦ᵣ inr ((pc_p,pc_g),pc_b,pc_e,a_cont)
+          ∗ r_self ↦ᵣ inr ((pc_p,pc_g),pc_b,pc_e,a_cont)
+          ∗ (∃ wsr, [∗ list] r_i;w_i ∈ list_difference all_registers [PC;r_self]; wsr, r_i ↦ᵣ w_i)
+          -∗ WP Seq (Instr Executable) {{ φ }})
+      ⊢ WP Seq (Instr Executable) {{ φ }})%I.
+     
+   
+   (* the following spec is for the f4 subroutine of the awkward example, jumped to after dynamically allocating into r_env *)
+   Lemma f4_spec W pc_p pc_g pc_b pc_e (* PC *)
+         b e a (* adv *)
+         f4_addrs flag_off (* f2 *)
+         d d' i (* dynamically allocated memory given by preamble, connected to invariant i *)
+         a_first a_last a_flag (* special adresses *) 
+         (b_r e_r b_r' : Addr) (* stack *) :
+    
+     (* PC assumptions *)
+     isCorrectPC (inr ((pc_p,pc_g),pc_b,pc_e,a_first)) ∧
+     isCorrectPC (inr ((pc_p,pc_g),pc_b,pc_e,a_last)) →
+     
+     (* Program adresses assumptions *)
+     contiguous f4_addrs ->
+     f4_addrs !! 0 = Some a_first ∧ list.last f4_addrs = Some a_last ->
+    
+     (* Stack assumptions *)
+     (0%a ≤ e_r)%Z ∧ (0%a ≤ b_r)%Z -> (* this assumption will not be necessary once addresses are finite *)
+     (b_r ≤ e_r)%Z ->
+     region_size b_r e_r > 12 -> (* we must assume the stack is large enough for needed local state *)
+     (b_r' + 1)%a = Some b_r ->
+
+     (* Preamble assumptions *)
+     (d + 1)%a = Some d' ->
+
+     (* Finally, we must assume that the stack is currently in a revoked state *)
+     Forall (λ a, revoked W a ∧ rel_is_std_i W (countable.encode a)) (region_addrs b_r e_r) ->
+
+     {{{ r_stk ↦ᵣ inr ((RWLX,Local),b_r,e_r,b_r')
+      ∗ PC ↦ᵣ inr ((pc_p,pc_g),pc_b,pc_e,a_first)
+      ∗ r_self ↦ᵣ inr ((pc_p,pc_g),pc_b,pc_e,a_first)
+      ∗ r_adv ↦ᵣ inr ((E,Global),b,e,a)
+      ∗ r_env ↦ᵣ inr (RWX,Global,d,d',d)
+      ∗ (∃ wsr, [∗ list] r_i;w_i ∈ list_difference all_registers [PC;r_stk;r_adv;r_self;r_env]; wsr, r_i ↦ᵣ w_i)
+      (* invariant for d *)
+      ∗ awk_inv i d
+      ∗ sts_rel_loc i awk_rel_pub awk_rel_priv
+      (* stack *)
+      ∗ (∃ ws, [[b_r, e_r]]↦ₐ[RWLX][[ws]])
+      (* flag *)
+      ∗ a_flag ↦ₐ[RW] inl 0%Z
+      (* token which states all non atomic invariants are closed *)
+      ∗ na_own logrel_nais ⊤
+      (* adv code *)
+      ∗ interp W (inr ((E,Global),b,e,a))
+      (* trusted code *)
+      ∗ awkward_example f4_addrs pc_p r_self r_adv 65 flag_off
+      (* we start out with arbitrary sts *)
+      ∗ sts_full_world sts_std W
+      ∗ region W
+    }}}
+      Seq (Instr Executable)
+    {{{ v, RET v; ⌜v = HaltedV⌝ → a_flag ↦ₐ[RW] inl 0%Z }}}.
+  Proof.
+                
+
    
 
 End awkward_example. 
